Various extensions.

checker/builtins.ml
@@ -1,4 +1,5 @@
 (* Registering parsers for coq csts *)
+module St = Stream
 module MT = MTypes
 module P = Parse
 module S = Spec
@@ -21,13 +22,19 @@ let string_of_list f ls =
     | (x :: xs) -> (f x) ^ "," ^ (aux xs)
   in "[" ^ (aux ls) ^ "]"
 
+let parse_iterm minfo toks =
+  match St.next toks with
+  | GL.Int k -> C_impl.Ilit k
+  | GL.Ident x -> C_impl.Ivar (Pr.get_ivar minfo x)
+  | _ -> failwith "Unexpected token in parse_iterm"
+
 let string_of_ints = string_of_list string_of_int
 
 (* Build the linear checker. *)
-let linear_args get_ivar = S.cons int_list (S.cons (ivar_list get_ivar) S.intconst)
+let linear_args get_ivar = S.cons int_list (S.cons (S.listof get_ivar) S.intconst)
 
 let minfo_parse_linear_le minfo tokens =
-   let (coeffs, (vars, k)) = linear_args (Pr.get_ivar minfo) tokens in
+   let (coeffs, (vars, k)) = linear_args (parse_iterm minfo) tokens in
    let linterms = List.map2 (fun c v -> (c, v)) coeffs vars in
    C_impl.make_linear linterms k
 
@@ -59,8 +66,8 @@ let minfo_parse_clause minfo toks =
 let parse_element minfo tokens =
   let (x, (i, ys)) =
     (S.cons
-      (parse_ivar (Pr.get_ivar minfo))
-      (S.cons (parse_ivar (Pr.get_ivar minfo)) int_list)) tokens in
+      (parse_iterm minfo)
+      (S.cons (parse_iterm minfo) (S.listof (parse_iterm minfo)))) tokens in
   C_impl.make_element x i ys
 
 let make_cumul xs durations resources lim =
@@ -104,11 +111,60 @@ let parse_disj model tokens =
   let y = Pr.parse_cst model tokens in
   C_impl.Disj (x, y)
 
+let parse_half model tokens =
+  let r = minfo_parse_lit model tokens in
+  chomp (GL.Kwd ",") tokens ;
+  let c = Pr.parse_cst model tokens in
+  C_impl.Half (r, c)
+
+let op_of_id id =
+  match id with
+  | "add" -> C_impl.Plus
+  | "mul" -> C_impl.Times
+  | "sub" -> C_impl.Sub
+  | "div" -> C_impl.Div
+  | "min" -> C_impl.Min
+  | "max" -> C_impl.Max
+  | _ -> failwith (Format.sprintf "Expected arithmetic operator, got %s" id)
+
+let rec parse_arith model tokens =
+  match St.next tokens with
+  | GL.Ident id ->
+    begin
+    match St.peek tokens with
+    | Some (GL.Kwd "(") ->
+      let _ = St.junk tokens in
+      let x = parse_arith model tokens in
+      chomp (GL.Kwd ",") tokens ;
+      let y = parse_arith model tokens in
+      chomp (GL.Kwd ")") tokens ;
+      C_impl.Op (op_of_id id, x, y)
+    | _ -> C_impl.T (C_impl.Ivar (Pr.get_ivar model id))
+    end
+  | GL.Int k -> C_impl.T (C_impl.Ilit k)
+  | _ -> failwith "Expected arithmetic expression"
+
+
+let parse_arith_eq model tokens =
+  let z = parse_iterm model tokens in
+  chomp (GL.Kwd ",") tokens ;
+  let exp = parse_arith model tokens in
+  C_impl.make_arith_eq z exp
+
+let parse_arith_ne model tokens =
+  let z = parse_iterm model tokens in
+  chomp (GL.Kwd ",") tokens ;
+  let exp = parse_arith model tokens in
+  C_impl.make_arith_ne z exp
+
 let register () =
   Pr.add_cst_parser "linear_le" minfo_parse_linear_le ;
   Pr.add_cst_parser "element" parse_element ;
   Pr.add_cst_parser "cumulative" parse_cumul ;
   Pr.add_cst_parser "clause" minfo_parse_clause ;
   Pr.add_cst_parser "and" parse_conj ;
-  Pr.add_cst_parser "or" parse_disj
+  Pr.add_cst_parser "or" parse_disj ;
+  Pr.add_cst_parser "half" parse_half ;
+  Pr.add_cst_parser "equal" parse_arith_eq ;
+  Pr.add_cst_parser "neq" parse_arith_ne
 
